iris/EscrowDeposit.v
@@ -114,7 +114,7 @@ Section EscrowDeposit.
     pose proof (islot_lt inum) as Hsl.
     assert (Hkey : (16 * Z.of_nat (ireg_bi inum) + Z.of_nat (islot inum))%Z
                    = bv_unsigned inum) by (symmetry; apply ireg_key_split).
-    iDestruct "Hinv" as "[#Hiinv #Hrb]".
+    iDestruct "Hinv" as "[#Hiinv [#Hrb #Hftopi]]".
     iMod (inv_acc E iregN with "Hiinv") as "[Hbody Hclose]"; [exact HE |].
     iDestruct "Hbody" as (m) "(>Ha & Hblks & >Hreg)".
     pose proof (ireg_bi_lt inum nib Hin) as Hbi.
