iris/IregLinkNz.v
@@ -83,7 +83,7 @@ Section IregLinkNz.
     pose proof (islot_lt inum) as Hsl.
     assert (Hkey : (16 * Z.of_nat (ireg_bi inum) + Z.of_nat (islot inum))%Z
                    = bv_unsigned inum) by (symmetry; apply ireg_key_split).
-    iDestruct "Hinv" as "[#Hiinv #Hrb]".
+    iDestruct "Hinv" as "[#Hiinv [#Hrb #Hftopi]]".
     iMod (inv_acc E iregN with "Hiinv") as "[Hbody Hclose]"; [exact HE |].
     iDestruct "Hbody" as (m) "(>Ha & Hblks & >Hreg)".
     pose proof (ireg_bi_lt inum nib Hin) as Hbi.
@@ -157,7 +157,7 @@ Section IregLinkNz.
     pose proof (islot_lt inum) as Hsl.
     assert (Hkey : (16 * Z.of_nat (ireg_bi inum) + Z.of_nat (islot inum))%Z
                    = bv_unsigned inum) by (symmetry; apply ireg_key_split).
-    iDestruct "Hinv" as "[#Hiinv #Hrb]".
+    iDestruct "Hinv" as "[#Hiinv [#Hrb #Hftopi]]".
     iMod (inv_acc E iregN with "Hiinv") as "[Hbody Hclose]"; [exact HE |].
     iDestruct "Hbody" as (m) "(>Ha & Hblks & >Hreg)".
     pose proof (ireg_bi_lt inum nib Hin) as Hbi.
@@ -195,7 +195,7 @@ Section IregLinkNz.
     pose proof (islot_lt inum) as Hsl.
     assert (Hkey : (16 * Z.of_nat (ireg_bi inum) + Z.of_nat (islot inum))%Z
                    = bv_unsigned inum) by (symmetry; apply ireg_key_split).
-    iDestruct "Hinv" as "[#Hiinv #Hrb]".
+    iDestruct "Hinv" as "[#Hiinv [#Hrb #Hftopi]]".
     iMod (inv_acc E iregN with "Hiinv") as "[Hbody Hclose]"; [exact HE |].
     iDestruct "Hbody" as (m) "(>Ha & Hblks & >Hreg)".
     pose proof (ireg_bi_lt inum nib Hin) as Hbi.
@@ -252,7 +252,7 @@ Section IregLinkNz.
     pose proof (islot_lt inum) as Hsl.
     assert (Hkey : (16 * Z.of_nat (ireg_bi inum) + Z.of_nat (islot inum))%Z
                    = bv_unsigned inum) by (symmetry; apply ireg_key_split).
-    iDestruct "Hinv" as "[#Hiinv #Hrb]".
+    iDestruct "Hinv" as "[#Hiinv [#Hrb #Hftopi]]".
     iMod (inv_acc E iregN with "Hiinv") as "[Hbody Hclose]"; [exact HE |].
     iDestruct "Hbody" as (m) "(>Ha & Hblks & >Hreg)".
     pose proof (ireg_bi_lt inum nib Hin) as Hbi.
@@ -314,7 +314,7 @@ Section IregLinkNz.
     pose proof (islot_lt inum) as Hsl.
     assert (Hkey : (16 * Z.of_nat (ireg_bi inum) + Z.of_nat (islot inum))%Z
                    = bv_unsigned inum) by (symmetry; apply ireg_key_split).
-    iDestruct "Hinv" as "[#Hiinv #Hrb]".
+    iDestruct "Hinv" as "[#Hiinv [#Hrb #Hftopi]]".
     iMod (inv_acc E iregN with "Hiinv") as "[Hbody Hclose]"; [exact HE |].
     iDestruct "Hbody" as (m) "(>Ha & Hblks & >Hreg)".
     pose proof (ireg_bi_lt inum nib Hin) as Hbi.
